misc_preprocessing.lean
@@ -10,7 +10,7 @@ return $ list.bor (do
 
 open tactic
 example (i : Type) (p : i → i → Type) (c : i) (h : ∀ (x : i), p x c → p x c) : true := by do
-h ← get_local `h, hcls ← monad.liftM (clause.mk 1 2 tt h) (infer_type h),
+h ← get_local `h, hcls ← clause.of_proof h,
 taut ← is_taut hcls,
 when (¬taut) failed,
 to_expr `(trivial) >>= apply
@@ -21,14 +21,3 @@ preprocessing_rule $ λnew, resolution_prover_of_tactic (filterM (λc, liftM bno
 meta def remove_duplicates_pre : resolution_prover unit :=
 preprocessing_rule $ λnew,
 return (rb_map.values (rb_map.of_list (list.map (λc:clause, (c↣type, c)) new)))
-
-meta def only_pos_to_fin_pre : resolution_prover unit :=
-preprocessing_rule $ take news, flip mapM news $ take new, do
-match list.filter (λl : (clause.literal × ℕ), l↣1↣is_pos) new↣get_lits↣zip_with_index with
-| [l] := do univ ← resolution_prover_of_tactic $ infer_univ l↣1↣formula,
-            if ¬l↣1↣is_final ∧ univ = level.zero then
-              resolution_prover_of_tactic (new↣focus l↣2)
-            else
-              return new
-| _ := return new
-end
