splitting.lean
@@ -11,17 +11,10 @@ else do
   hd ← return $ c↣get_lit 0,
   hyp_opt ← get_sat_hyp_core hd↣formula hd↣is_neg,
   match hyp_opt with
-  | some h :=
-    if hd↣is_final then do
-      c' ← resolution_prover_of_tactic c↣fin_to_pos,
-      return (c'↣inst h, [h])
-    else do
+  | some h := do
       wo_as ← extract_assertions (c↣inst h),
       return (wo_as↣1, h :: wo_as↣2)
-  | _ :=
-    if hd↣is_final then
-      return (c, [])
-    else do
+  | _ := do
       op ← resolution_prover_of_tactic c↣open_const,
       op_wo_as ← extract_assertions op↣1,
       return (op_wo_as↣1↣close_const op↣2, op_wo_as↣2)
